Iris/Iris/ProgramLogic/Lifting.lean
@@ -184,7 +184,7 @@ theorem wp_lift_pure_det_step_no_fork [Inhabited State] (E₂ : CoPset)
 
 @[rocq_alias wp_pure_step_fupd]
 theorem wp_pure_step_fupd [Inhabited State] (E₂ : CoPset)
-    (Hexec : PureExec φ n e₁ e₂) (Hφ : φ) :
+    [Hexec : PureExec φ n e₁ e₂] (Hφ : φ) :
     (|={E}[E₂]▷=>^[n] £ n -∗ WP e₂ @ s; E {{ Φ }}) ⊢ WP e₁ @ s; E {{ Φ }} := by
   iintro Hwp
   replace Hexec := Hexec.pureExec Hφ
@@ -212,9 +212,9 @@ theorem wp_pure_step_fupd [Inhabited State] (E₂ : CoPset)
     iframe
 
 @[rocq_alias wp_pure_step_later]
-theorem wp_pure_step_later [Inhabited State] (Hexec : PureExec φ n e₁ e₂) (Hφ : φ) :
+theorem wp_pure_step_later [Inhabited State] [Hexec : PureExec φ n e₁ e₂] (Hφ : φ) :
     ▷^[n] (£ n -∗ WP e₂ @ s; E {{ Φ }}) ⊢ WP e₁ @ s; E {{ Φ }} := by
-  refine .trans ?_  (wp_pure_step_fupd E Hexec Hφ)
+  refine .trans ?_  (wp_pure_step_fupd E Hφ)
   suffices Hwp : ∀ (P : IProp GF), ▷^[n] P ⊢ |={E}▷=>^[n] P by iapply Hwp
   intro P
   clear Hexec
